pulse/lib/steel/pulse/Pulse.Typing.Metatheory.fst
@@ -1,0 +1,14 @@
+module Pulse.Typing.Metatheory
+open Pulse.Syntax
+open Pulse.Typing
+
+let st_typing_correctness (#g:env) (#t:st_term) (#c:comp_st) 
+                          (_:st_typing g t c)
+  : comp_typing_u g c
+  = admit()
+
+let add_frame_well_typed (#g:env) (#c:comp_st) (ct:comp_typing_u g c)
+                         (#f:term) (ft:tot_typing g f Tm_VProp)
+  : comp_typing_u g (add_frame c f)
+  = admit()
+
